Change rec domain eq to `proto = 1 + (action * ▶ (V → proto → PROP))`.
By moving the later further to the outside, we can kill many occurences
of `Next`, and get rid of laters/except_0s at awkward positions. Also we
can have a sensible eliminator `proto_elim`.

theories/channel/proto.v
@@ -58,10 +58,9 @@ Arguments iProto_end {_ _}.
 Program Definition iProto_message_def {Σ V} {TT : tele} (a : action)
     (pc : TT → V * iProp Σ * iProto Σ V) : iProto Σ V :=
   proto_message a (λ v, λne p', ∃ x : TT,
-    (** We need the later to make [iProto_message] contractive *)
     ⌜ v = (pc x).1.1 ⌝ ∗
-    ▷ (pc x).1.2 ∗
-    p' ≡ Next (pc x).2)%I.
+    (pc x).1.2 ∗
+    p' ≡ (pc x).2)%I.
 Next Obligation. solve_proper. Qed.
 Definition iProto_message_aux : seal (@iProto_message_def). by eexists. Qed.
 Definition iProto_message := iProto_message_aux.(unseal).
@@ -146,31 +145,29 @@ Notation "<?> 'MSG' v ; p" :=
 Notation "'END'" := iProto_end : proto_scope.
 
 (** * Operations *)
-Program Definition iProto_map_cont {Σ V}
-    (rec : iProto Σ V → iProto Σ V) (pc : laterO (iProto Σ V) -n> iPropO Σ) :
-    laterO (iProto Σ V) -n> iPropO Σ :=
-  λne p2, (∃ p1, pc (Next p1) ∗ p2 ≡ Next (rec p1))%I.
+Program Definition iProto_map_app_cont {Σ V}
+    (rec : iProto Σ V → iProto Σ V) (pc : iProto Σ V -n> iPropO Σ) :
+    iProto Σ V -n> iPropO Σ :=
+  λne p1', (∃ p1, pc p1 ∗ p1' ≡ rec p1)%I.
 Next Obligation. solve_proper. Qed.
 
 Program Definition iProto_map_app_aux {Σ V}
     (f : action → action) (p2 : iProto Σ V)
-    (rec : iProto Σ V -n> iProto Σ V) : iProto Σ V -n> iProto Σ V := λne p1,
-  match proto_unfold p1 return _ with
-  | None => p2
-  | Some (a, pc) => proto_message (f a) (iProto_map_cont rec ∘ pc)
-  end.
+    (rec : iProto Σ V -n> iProto Σ V) : iProto Σ V -n> iProto Σ V := λne p,
+  proto_elim p2 (λ a pc,
+    proto_message (f a) (iProto_map_app_cont rec ∘ pc)) p.
 Next Obligation.
-  intros Σ V f p2 rec n p1 p1'
-    [[??][??] [-> Hf]|]%(ofe_mor_ne _ _ proto_unfold); last done.
-  f_equiv=> v pc; rewrite /= /iProto_map_cont /=. by repeat f_equiv.
+  intros Σ V f p2 rec n p1 p1' Hp. apply proto_elim_ne=> // a pc1 pc2 Hpc.
+  apply proto_message_contractive; destruct n as [|n]=> // v p'; simpl in *.
+  by repeat f_equiv.
 Qed.
 
 Instance iProto_map_app_aux_contractive {Σ V} f (p2 : iProto Σ V) :
   Contractive (iProto_map_app_aux f p2).
 Proof.
-  intros n rec1 rec2 Hrec p1. simpl.
-  destruct (proto_unfold p1) as [[a c]|]; last done.
-  f_equiv=> v p' /=. by repeat (f_contractive || f_equiv).
+  intros n rec1 rec2 Hrec p1; simpl. apply proto_elim_ne=> // a pc1 pc2 Hpc.
+  apply proto_message_contractive; destruct n as [|n]=> // v p'; simpl in *.
+  by repeat f_equiv.
 Qed.
 
 Definition iProto_map_app {Σ V} (f : action → action)
@@ -179,7 +176,7 @@ Definition iProto_map_app {Σ V} (f : action → action)
 
 Definition iProto_app_def {Σ V} (p1 p2 : iProto Σ V) : iProto Σ V :=
   iProto_map_app id p2 p1.
-Definition iProto_app_aux : seal (@iProto_app_def). by eexists. Qed.
+Definition iProto_app_aux : seal (@iProto_app_def). Proof. by eexists. Qed.
 Definition iProto_app := iProto_app_aux.(unseal).
 Definition iProto_app_eq : @iProto_app = @iProto_app_def := iProto_app_aux.(seal_eq).
 Arguments iProto_app {_ _} _%proto _%proto.
@@ -188,7 +185,7 @@ Infix "<++>" := iProto_app (at level 60) : proto_scope.
 
 Definition iProto_dual_def {Σ V} (p : iProto Σ V) : iProto Σ V :=
   iProto_map_app action_dual proto_end p.
-Definition iProto_dual_aux : seal (@iProto_dual_def). by eexists. Qed.
+Definition iProto_dual_aux : seal (@iProto_dual_def). Proof. by eexists. Qed.
 Definition iProto_dual := iProto_dual_aux.(unseal).
 Definition iProto_dual_eq :
   @iProto_dual = @iProto_dual_def := iProto_dual_aux.(seal_eq).
@@ -226,20 +223,14 @@ Definition iProto_le_pre {Σ V}
     p1 ≡ proto_message a1 pc1 ∗
     p2 ≡ proto_message a2 pc2 ∗
     match a1, a2 with
-    | Recv, Recv =>
-       ∀ v p1', pc1 v (Next p1') -∗
-         ◇ ∃ p2', ▷ rec p1' p2' ∗ pc2 v (Next p2')
-    | Send, Send =>
-       ∀ v p2', pc2 v (Next p2') -∗
-         ◇ ∃ p1', ▷ rec p1' p2' ∗ pc1 v (Next p1')
-    | Recv, Send =>
-       ∀ v1 v2 p1' p2',
-         pc1 v1 (Next p1') -∗ pc2 v2 (Next p2') -∗
-         ◇ ∃ pc1' pc2' pt,
-           ▷ rec p1' (proto_message Send pc1') ∗
-           ▷ rec (proto_message Recv pc2') p2' ∗
-           pc1' v2 (Next pt) ∗
-           pc2' v1 (Next pt)
+    | Recv, Recv => ▷ ∀ v p1', pc1 v p1' -∗ ∃ p2', rec p1' p2' ∗ pc2 v p2'
+    | Send, Send => ▷ ∀ v p2', pc2 v p2' -∗ ∃ p1', rec p1' p2' ∗ pc1 v p1'
+    | Recv, Send => ▷ ∀ v1 v2 p1' p2',
+       pc1 v1 p1' -∗ pc2 v2 p2' -∗ ∃ pc1' pc2' pt,
+         rec p1' (proto_message Send pc1') ∗
+         rec (proto_message Recv pc2') p2' ∗
+         pc1' v2 pt ∗
+         pc2' v1 pt
     | Send, Recv => False
     end.
 Instance iProto_le_pre_ne {Σ V} (rec : iProto Σ V → iProto Σ V → iProp Σ) :
@@ -248,8 +239,8 @@ Proof. solve_proper. Qed.
 
 Program Definition iProto_le_pre' {Σ V}
     (rec : iProto Σ V -n> iProto Σ V -n> iPropO Σ) :
-    iProto Σ V -n> iProto Σ V -n> iPropO Σ :=
-  λne p1 p2, iProto_le_pre (λ p1' p2', rec p1' p2') p1 p2.
+    iProto Σ V -n> iProto Σ V -n> iPropO Σ := λne p1 p2,
+  iProto_le_pre (λ p1' p2', rec p1' p2') p1 p2.
 Solve Obligations with solve_proper.
 Local Instance iProto_le_pre_contractive {Σ V} : Contractive (@iProto_le_pre' Σ V).
 Proof.
@@ -273,12 +264,12 @@ Fixpoint iProto_interp_aux {Σ V} (n : nat)
      (∃ vl vsl' pc p2',
        ⌜ vsl = vl :: vsl' ⌝ ∗
        iProto_le (proto_message Recv pc) pr ∗
-       pc vl (Next p2') ∗
+       pc vl p2' ∗
        iProto_interp_aux n vsl' vsr pl p2') ∨
      (∃ vr vsr' pc p1',
        ⌜ vsr = vr :: vsr' ⌝ ∗
        iProto_le (proto_message Recv pc) pl ∗
-       pc vr (Next p1') ∗
+       pc vr p1' ∗
        iProto_interp_aux n vsl vsr' p1' pr)
   end.
 Definition iProto_interp {Σ V} (vsl vsr : list V) (pl pr : iProto Σ V) : iProp Σ :=
@@ -347,7 +338,7 @@ Section proto.
   Proof.
     rewrite !tforall_forall=> Hv HP Hp.
     rewrite iProto_message_eq /iProto_message_def.
-    f_equiv=> v f /=. apply bi.exist_ne=> x.
+    apply proto_message_contractive; destruct n as [|n]=> // v f /=.
     repeat (apply Hv || apply HP || apply Hp || f_contractive || f_equiv).
   Qed.
   Lemma iProto_message_ne {TT} a (pc1 pc2 : TT → V * iProp Σ * iProto Σ V) n :
@@ -383,23 +374,16 @@ Section proto.
   Lemma iProto_dual_end' : iProto_dual (Σ:=Σ) (V:=V) proto_end ≡ proto_end.
   Proof.
     rewrite iProto_dual_eq /iProto_dual_def /iProto_map_app.
-    etrans; [eapply (fixpoint_unfold (iProto_map_app_aux _ _))|]; simpl.
-    pose proof (proto_unfold_fold (V:=V)
-      (PROP:=iPropO Σ) (PROPn:=iPropO Σ) None) as Hfold.
-    by destruct (proto_unfold (proto_fold None))
-      as [[??]|] eqn:E; rewrite E; inversion Hfold.
+    etrans; [apply (fixpoint_unfold (iProto_map_app_aux _ _))|]; simpl.
+    by rewrite proto_elim_end.
   Qed.
   Lemma iProto_dual_message' a pc :
     iProto_dual (Σ:=Σ) (V:=V) (proto_message a pc)
-    ≡ proto_message (action_dual a) (iProto_map_cont iProto_dual ∘ pc).
+    ≡ proto_message (action_dual a) (iProto_map_app_cont iProto_dual ∘ pc).
   Proof.
-    rewrite iProto_dual_eq /iProto_dual_def /iProto_map_app /proto_message.
-    etrans; [eapply (fixpoint_unfold (iProto_map_app_aux _ _))|]; simpl.
-    pose proof (proto_unfold_fold (V:=V) (PROP:=iPropO Σ)
-      (PROPn:=iPropO Σ) (Some (a,pc))) as Hfold.
-    destruct (proto_unfold (proto_fold (Some (a, pc))))
-      as [[??]|] eqn:E; inversion Hfold as [?? [Ha Hpc]|]; simplify_eq/=.
-    rewrite /proto_message. do 3 f_equiv; intros v p'; simpl. by repeat f_equiv.
+    rewrite iProto_dual_eq /iProto_dual_def /iProto_map_app.
+    etrans; [apply (fixpoint_unfold (iProto_map_app_aux _ _))|]; simpl.
+    apply: proto_elim_message=> a' pc1 pc2 Hpc; f_equiv; solve_proper.
   Qed.
 
   Lemma iProto_dual_end : iProto_dual (Σ:=Σ) (V:=V) END ≡ END%proto.
@@ -412,7 +396,7 @@ Section proto.
     rewrite iProto_message_eq /iProto_message_def iProto_dual_message' /=.
     do 2 f_equiv; intros p'; simpl. iSplit.
     - iDestruct 1 as (pd) "[H Hp']". iDestruct "H" as (x ->) "[Hpc Hpd]".
-      iExists x. iSplit; [done|]; iFrame. iRewrite "Hp'". iNext. by iRewrite "Hpd".
+      iExists x. iSplit; [done|]; iFrame. iRewrite "Hp'". by iRewrite "Hpd".
     - iDestruct 1 as (x ->) "[Hpc Hpd]"; auto 10.
   Qed.
 
@@ -423,36 +407,27 @@ Section proto.
     { by rewrite !iProto_dual_end'. }
     rewrite !iProto_dual_message' involutive.
     iApply proto_message_equivI; iSplit; [done|]; iIntros (v p') "/=".
-    iApply prop_ext; iIntros "!>"; iSplit.
+    iIntros "!>"; iApply prop_ext; iIntros "!>"; iSplit.
     - iDestruct 1 as (pd) "[H Hp']". iRewrite "Hp'".
-      iDestruct "H" as (pdd) "[H #Hpd]".
-      iApply (bi.internal_eq_rewrite); [|done]; iModIntro.
-      iRewrite "Hpd". by iRewrite ("IH" $! pdd).
-    - iIntros "H". destruct (Next_uninj p') as [p'' Hp']. iExists (iProto_dual p'').
-      rewrite Hp'. iSplitL; [by auto|]. iNext. by iRewrite ("IH" $! p'').
+      iDestruct "H" as (pdd) "[H Hpd]". iRewrite "Hpd". by iRewrite ("IH" $! pdd).
+    - iIntros "H". iExists (iProto_dual p').
+      iSplitL; [by auto|]. by iRewrite ("IH" $! p').
   Qed.
 
   (** ** Append *)
   Lemma iProto_app_end' p : (proto_end <++> p)%proto ≡ p.
   Proof.
     rewrite iProto_app_eq /iProto_app_def /iProto_map_app.
-    etrans; [eapply (fixpoint_unfold (iProto_map_app_aux _ _))|]; simpl.
-    pose proof (proto_unfold_fold (V:=V)
-      (PROP:=iPropO Σ) (PROPn:=iPropO Σ) None) as Hfold.
-    by destruct (proto_unfold (proto_fold None))
-      as [[??]|] eqn:E; rewrite E; inversion Hfold.
+    etrans; [apply (fixpoint_unfold (iProto_map_app_aux _ _))|]; simpl.
+    by rewrite proto_elim_end.
   Qed.
   Lemma iProto_app_message' a pc p2 :
     (proto_message a pc <++> p2)%proto
-    ≡ proto_message a (iProto_map_cont (flip iProto_app p2) ∘ pc).
+    ≡ proto_message a (iProto_map_app_cont (flip iProto_app p2) ∘ pc).
   Proof.
-    rewrite iProto_app_eq /iProto_app_def /iProto_map_app /proto_message.
-    etrans; [eapply (fixpoint_unfold (iProto_map_app_aux _ _))|]; simpl.
-    pose proof (proto_unfold_fold (V:=V) (PROP:=iPropO Σ)
-      (PROPn:=iPropO Σ) (Some (a,pc))) as Hfold.
-    destruct (proto_unfold (proto_fold (Some (a, pc))))
-      as [[??]|] eqn:E; inversion Hfold as [?? [Ha Hpc]|]; simplify_eq/=.
-    rewrite /proto_message. do 3 f_equiv; intros v p'; simpl. by repeat f_equiv.
+    rewrite iProto_app_eq /iProto_app_def /iProto_map_app.
+    etrans; [apply (fixpoint_unfold (iProto_map_app_aux _ _))|]; simpl.
+    apply: proto_elim_message => a' pc1 pc2 Hpc. f_equiv; solve_proper.
   Qed.
 
   Global Instance iProto_app_ne : NonExpansive2 (@iProto_app Σ V).
@@ -465,8 +440,9 @@ Section proto.
     revert p1'. induction (lt_wf n) as [n _ IH]; intros p1.
     destruct (proto_case p1) as [->|(a&pc&->)].
     { by rewrite !iProto_app_end'. }
-    rewrite !iProto_app_message'. f_equiv=> v p' /=. f_equiv=> p12.
-    do 2 f_equiv. f_contractive. apply IH; eauto using dist_le with lia.
+    rewrite !iProto_app_message'.
+    apply proto_message_contractive; destruct n as [|n]=> // v p' /=.
+    do 4 f_equiv. apply IH; eauto using dist_le with lia.
   Qed.
   Global Instance iProto_app_proper : Proper ((≡) ==> (≡) ==> (≡)) (@iProto_app Σ V).
   Proof. apply (ne_proper_2 _). Qed.
@@ -478,7 +454,7 @@ Section proto.
     rewrite iProto_message_eq /iProto_message_def iProto_app_message' /=.
     f_equiv=> v ps /=. iSplit.
     - iDestruct 1 as (p1') "[H Hps]". iDestruct "H" as (x ->) "[Hpc #Hp1']".
-      iExists x. iSplit; [done|]. iFrame. iRewrite "Hps". iNext. by iRewrite "Hp1'".
+      iExists x. iSplit; [done|]. iFrame. iRewrite "Hps". by iRewrite "Hp1'".
     - iDestruct 1 as (x ->) "[Hpc Hps]". auto 10.
   Qed.
 
@@ -492,12 +468,9 @@ Section proto.
     { by rewrite iProto_app_end'. }
     rewrite iProto_app_message'.
     iApply proto_message_equivI; iSplit; [done|]; iIntros (v p') "/=".
-    iApply prop_ext; iIntros "!>". iSplit.
-    - iDestruct 1 as (p1') "[H Hp']". iRewrite "Hp'".
-      iApply (bi.internal_eq_rewrite); [|done]; iModIntro.
-      by iRewrite ("IH" $! p1').
-    - iIntros "H". destruct (Next_uninj p') as [p'' Hp']. iExists p''.
-      rewrite Hp'. iFrame "H". iNext. by iRewrite ("IH" $! p'').
+    iIntros "!>". iApply prop_ext; iIntros "!>". iSplit.
+    - iDestruct 1 as (p1') "[H Hp']". iRewrite "Hp'". by iRewrite ("IH" $! p1').
+    - iIntros "H". iExists p'. iFrame "H". by iRewrite ("IH" $! p').
   Qed.
   Global Instance iProto_app_assoc : Assoc (≡) (@iProto_app Σ V).
   Proof.
@@ -506,13 +479,13 @@ Section proto.
     { by rewrite !iProto_app_end'. }
     rewrite !iProto_app_message'.
     iApply proto_message_equivI; iSplit; [done|]; iIntros (v p123) "/=".
-    iApply prop_ext; iIntros "!>". iSplit.
+    iIntros "!>". iApply prop_ext; iIntros "!>". iSplit.
     - iDestruct 1 as (p1') "[H #Hp']".
       iExists (p1' <++> p2)%proto. iSplitL; [by auto|].
-      iRewrite "Hp'". iNext. iApply "IH".
+      iRewrite "Hp'". iApply "IH".
     - iDestruct 1 as (p12) "[H #Hp123]". iDestruct "H" as (p1') "[H #Hp12]".
       iExists p1'. iFrame "H". iRewrite "Hp123".
-      iNext. iRewrite "Hp12". by iRewrite ("IH" $! p1').
+      iRewrite "Hp12". by iRewrite ("IH" $! p1').
   Qed.
 
   Lemma iProto_dual_app p1 p2 :
@@ -523,13 +496,13 @@ Section proto.
     { by rewrite iProto_dual_end' !iProto_app_end'. }
     rewrite iProto_dual_message' !iProto_app_message' iProto_dual_message' /=.
     iApply proto_message_equivI; iSplit; [done|]; iIntros (v p12) "/=".
-    iApply prop_ext; iIntros "!>". iSplit.
+    iIntros "!>"; iApply prop_ext; iIntros "!>". iSplit.
     - iDestruct 1 as (p12d) "[H #Hp12]". iDestruct "H" as (p1') "[H #Hp12d]".
       iExists (iProto_dual p1'). iSplitL; [by auto|].
-      iRewrite "Hp12". iNext. iRewrite "Hp12d". iApply "IH".
+      iRewrite "Hp12". iRewrite "Hp12d". iApply "IH".
     - iDestruct 1 as (p1') "[H #Hp12]". iDestruct "H" as (p1d) "[H #Hp1']".
       iExists (p1d <++> p2)%proto. iSplitL; [by auto|].
-      iRewrite "Hp12". iNext. iRewrite "Hp1'". by iRewrite ("IH" $! p1d p2).
+      iRewrite "Hp12". iRewrite "Hp1'". by iRewrite ("IH" $! p1d p2).
   Qed.
 
   (** ** Protocol entailment **)
@@ -546,9 +519,9 @@ Section proto.
     iLöb as "IH" forall (p). destruct (proto_case p) as [->|([]&pc&->)].
     - rewrite iProto_le_unfold. iLeft; by auto.
     - rewrite iProto_le_unfold. iRight. iExists _, _, _, _; do 2 (iSplit; [done|]).
-      iIntros (v p') "Hpc". iExists p'. iIntros "{$Hpc} !> !>". iApply "IH".
+      iIntros "!>" (v p') "Hpc". iExists p'. iFrame "Hpc". iApply "IH".
     - rewrite iProto_le_unfold. iRight. iExists _, _, _, _; do 2 (iSplit; [done|]).
-      iIntros (v p') "Hpc". iExists p'. iIntros "{$Hpc} !> !>". iApply "IH".
+      iIntros "!>" (v p') "Hpc". iExists p'. iFrame "Hpc". iApply "IH".
   Qed.
 
   Lemma iProto_le_end_inv p : iProto_le p proto_end -∗ p ≡ proto_end.
@@ -562,17 +535,13 @@ Section proto.
     iProto_le p1 (proto_message Send pc2) -∗ ∃ a1 pc1,
       p1 ≡ proto_message a1 pc1 ∗
       match a1 with
-      | Send =>
-         ∀ v p2', pc2 v (Next p2') -∗
-           ◇ ∃ p1', ▷ iProto_le p1' p2' ∗ pc1 v (Next p1')
-      | Recv =>
-         ∀ v1 v2 p1' p2',
-           pc1 v1 (Next p1') -∗ pc2 v2 (Next p2') -∗
-           ◇ ∃ pc1' pc2' pt,
-             ▷ iProto_le p1' (proto_message Send pc1') ∗
-             ▷ iProto_le (proto_message Recv pc2') p2' ∗
-             pc1' v2 (Next pt) ∗
-             pc2' v1 (Next pt)
+      | Send => ▷ ∀ v p2', pc2 v p2' -∗ ∃ p1', iProto_le p1' p2' ∗ pc1 v p1'
+      | Recv => ▷ ∀ v1 v2 p1' p2',
+         pc1 v1 p1' -∗ pc2 v2 p2' -∗ ∃ pc1' pc2' pt,
+           iProto_le p1' (proto_message Send pc1') ∗
+           iProto_le (proto_message Recv pc2') p2' ∗
+           pc1' v2 pt ∗
+           pc2' v1 pt
       end.
   Proof.
     rewrite iProto_le_unfold. iIntros "[[_ Heq]|H]".
@@ -580,23 +549,22 @@ Section proto.
     iDestruct "H" as (a1 a2 pc1 pc2') "(Hp1 & Hp2 & H)".
     iDestruct (proto_message_equivI with "Hp2") as (<-) "{Hp2} #Hpc".
     iExists _, _; iSplit; [done|]. destruct a1.
-    - iIntros (v p2'). by iRewrite ("Hpc" $! v (Next p2')).
-    - iIntros (v1 v2 p1' p2'). by iRewrite ("Hpc" $! v2 (Next p2')).
+    - iIntros "!>" (v p2'). by iRewrite ("Hpc" $! v p2').
+    - iIntros "!>" (v1 v2 p1' p2'). by iRewrite ("Hpc" $! v2 p2').
   Qed.
 
   Lemma iProto_le_recv_inv p1 pc2 :
     iProto_le p1 (proto_message Recv pc2) -∗ ∃ pc1,
       p1 ≡ proto_message Recv pc1 ∗
-      ∀ v p1', pc1 v (Next p1') -∗
-        ◇ ∃ p2', ▷ iProto_le p1' p2' ∗ pc2 v (Next p2').
+      ▷ ∀ v p1', pc1 v p1' -∗ ∃ p2', iProto_le p1' p2' ∗ pc2 v p2'.
   Proof.
     rewrite iProto_le_unfold. iIntros "[[_ Heq]|H]".
     { by iDestruct (proto_message_end_equivI with "Heq") as %[]. }
     iDestruct "H" as (a1 a2 pc1 pc2') "(Hp1 & Hp2 & H)".
     iDestruct (proto_message_equivI with "Hp2") as (<-) "{Hp2} #Hpc2".
     destruct a1; [done|]. iExists _; iSplit; [done|].
-    iIntros (v p1') "Hpc". iDestruct ("H" with "Hpc") as (p2') ">[Hle Hpc]".
-    iExists p2'. iFrame "Hle". by iRewrite ("Hpc2" $! v (Next p2')).
+    iIntros "!>" (v p1') "Hpc". iDestruct ("H" with "Hpc") as (p2') "[Hle Hpc]".
+    iExists p2'. iFrame "Hle". by iRewrite ("Hpc2" $! v p2').
   Qed.
 
   Lemma iProto_le_trans p1 p2 p3 :
@@ -610,53 +578,33 @@ Section proto.
       + iDestruct (iProto_le_send_inv with "H1") as (a1 pc1) "[Hp1 H1]".
         iRewrite "Hp1"; clear p1. rewrite iProto_le_unfold; iRight.
         iExists _, _, _, _; do 2 (iSplit; [done|]). destruct a1.
-        * iIntros (v p3') "Hpc".
-          iMod ("H2" with "Hpc") as (p2') "[Hle Hpc]".
-          iMod ("H1" with "Hpc") as (p1') "[Hle' Hpc]".
-          iExists p1'. iIntros "{$Hpc} !>". by iApply ("IH" with "Hle'").
-        * iIntros (v1 v3 p1' p3') "Hpc1 Hpc3".
-          iMod ("H2" with "Hpc3") as (p2') "[Hle Hpc2]".
-          iMod ("H1" with "Hpc1 Hpc2") as (pc1' pc2' pt) "(Hp1' & Hp2' & Hpc)".
-          iModIntro. iExists pc1', pc2', pt. iFrame "Hp1' Hpc".
-          by iApply ("IH" with "Hp2'").
+        * iIntros "!>" (v p3') "Hpc".
+          iDestruct ("H2" with "Hpc") as (p2') "[Hle Hpc]".
+          iDestruct ("H1" with "Hpc") as (p1') "[Hle' Hpc]".
+          iExists p1'. iFrame "Hpc". by iApply ("IH" with "Hle'").
+        * iIntros "!>" (v1 v3 p1' p3') "Hpc1 Hpc3".
+          iDestruct ("H2" with "Hpc3") as (p2') "[Hle Hpc2]".
+          iDestruct ("H1" with "Hpc1 Hpc2") as (pc1' pc2' pt) "(Hp1' & Hp2' & Hpc)".
+          iExists pc1', pc2', pt. iFrame "Hp1' Hpc". by iApply ("IH" with "Hp2'").
       + iDestruct (iProto_le_recv_inv with "H1") as (pc1) "[Hp1 H1]".
         iRewrite "Hp1"; clear p1. rewrite iProto_le_unfold; iRight.
         iExists _, _, _, _; do 2 (iSplit; [done|]); simpl.
-        iIntros (v1 v3 p1' p3') "Hpc1 Hpc3".
-        iMod ("H1" with "Hpc1") as (p2') "[Hle Hpc2]".
-        iMod ("H2" with "Hpc2 Hpc3") as (pc2' pc3' pt) "(Hp2' & Hp3' & Hpc)".
-        iModIntro. iExists pc2', pc3', pt. iFrame "Hp3' Hpc".
-        by iApply ("IH" with "Hle").
+        iIntros "!>" (v1 v3 p1' p3') "Hpc1 Hpc3".
+        iDestruct ("H1" with "Hpc1") as (p2') "[Hle Hpc2]".
+        iDestruct ("H2" with "Hpc2 Hpc3") as (pc2' pc3' pt) "(Hp2' & Hp3' & Hpc)".
+        iExists pc2', pc3', pt. iFrame "Hp3' Hpc". by iApply ("IH" with "Hle").
     - iDestruct (iProto_le_recv_inv with "H2") as (pc2) "[Hp2 H3]".
       iRewrite "Hp2" in "H1".
       iDestruct (iProto_le_recv_inv with "H1") as (pc1) "[Hp1 H2]".
       iRewrite "Hp1". rewrite iProto_le_unfold. iRight.
       iExists _, _, _, _; do 2 (iSplit; [done|]).
-      iIntros (v p1') "Hpc".
-      iMod ("H2" with "Hpc") as (p2') "[Hle Hpc]".
-      iMod ("H3" with "Hpc") as (p3') "[Hle' Hpc]".
-      iModIntro. iExists p3'. iIntros "{$Hpc} !>". by iApply ("IH" with "Hle").
+      iIntros "!>" (v p1') "Hpc".
+      iDestruct ("H2" with "Hpc") as (p2') "[Hle Hpc]".
+      iDestruct ("H3" with "Hpc") as (p3') "[Hle' Hpc]".
+      iExists p3'. iFrame "Hpc". by iApply ("IH" with "Hle").
   Qed.
 
   Lemma iProto_le_send {TT1 TT2} (pc1 : TT1 → V * iProp Σ * iProto Σ V)
-      (pc2 : TT2 → V * iProp Σ * iProto Σ V) :
-    (∀.. x2 : TT2, ▷ (pc2 x2).1.2 -∗ ◇ ∃.. x1 : TT1,
-      ⌜(pc1 x1).1.1 = (pc2 x2).1.1⌝ ∗
-      ▷ (pc1 x1).1.2 ∗
-      ▷ iProto_le (pc1 x1).2 (pc2 x2).2) -∗
-    iProto_le (iProto_message Send pc1) (iProto_message Send pc2).
-  Proof.
-    iIntros "H". rewrite iProto_le_unfold iProto_message_eq.
-    iRight. iExists _, _, _, _; do 2 (iSplit; [done|]).
-    iIntros (v p2') "/=". iDestruct 1 as (x2 ->) "[Hpc #Heq]".
-    iMod ("H" with "Hpc") as (x1 ?) "[Hpc Hle]".
-    iModIntro. iExists (pc1 x1).2. iSplitL "Hle".
-    { iIntros "!>". by iRewrite "Heq". }
-    iExists x1. iSplit; [done|]. iSplit; [by iApply "Hpc"|done].
-  Qed.
-  (* The following derived rule is weaker, but the positions of the laters
-  make more sense intuitively and practically. *)
-  Lemma iProto_le_send' {TT1 TT2} (pc1 : TT1 → V * iProp Σ * iProto Σ V)
       (pc2 : TT2 → V * iProp Σ * iProto Σ V) :
     ▷ (∀.. x2 : TT2, (pc2 x2).1.2 -∗ ∃.. x1 : TT1,
       ⌜(pc1 x1).1.1 = (pc2 x2).1.1⌝ ∗
@@ -664,28 +612,15 @@ Section proto.
       iProto_le (pc1 x1).2 (pc2 x2).2) -∗
     iProto_le (iProto_message Send pc1) (iProto_message Send pc2).
   Proof.
-    iIntros "H". iApply iProto_le_send. iIntros (x2) "Hpc".
-    rewrite bi_tforall_forall. iDestruct ("H" with "Hpc") as "H".
-    rewrite bi_texist_exist bi.later_exist_except_0.
-    iMod "H" as (x1) "(>% & Hpc & Hle)". iExists x1. by iFrame.
+    iIntros "H". rewrite iProto_le_unfold iProto_message_eq.
+    iRight. iExists _, _, _, _; do 2 (iSplit; [done|]).
+    iIntros "!>" (v p2') "/=". iDestruct 1 as (x2 ->) "[Hpc #Heq]".
+    iDestruct ("H" with "Hpc") as (x1 ?) "[Hpc Hle]".
+    iExists (pc1 x1).2. iSplitL "Hle"; [by iRewrite "Heq"|].
+    iExists x1. iSplit; [done|]. iSplit; [by iApply "Hpc"|done].
   Qed.
 
   Lemma iProto_le_recv {TT1 TT2} (pc1 : TT1 → V * iProp Σ * iProto Σ V)
-      (pc2 : TT2 → V * iProp Σ * iProto Σ V) :
-    (∀.. x1 : TT1, ▷ (pc1 x1).1.2 -∗ ◇ ∃.. x2 : TT2,
-      ⌜(pc1 x1).1.1 = (pc2 x2).1.1⌝ ∗
-      ▷ (pc2 x2).1.2 ∗
-      ▷ iProto_le (pc1 x1).2 (pc2 x2).2) -∗
-    iProto_le (iProto_message Recv pc1) (iProto_message Recv pc2).
-  Proof.
-    iIntros "H". rewrite iProto_le_unfold iProto_message_eq.
-    iRight. iExists _, _, _, _; do 2 (iSplit; [done|]).
-    iIntros (v p1') "/=". iDestruct 1 as (x1 ->) "[Hpc #Heq]".
-    iMod ("H" with "Hpc") as (x2 ?) "[Hpc Hle]". iExists (pc2 x2).2. iSplitL "Hle".
-    { iIntros "!> !>". by iRewrite "Heq". }
-    iModIntro. iExists x2. iSplit; [done|]. iSplit; [by iApply "Hpc"|done].
-  Qed.
-  Lemma iProto_le_recv' {TT1 TT2} (pc1 : TT1 → V * iProp Σ * iProto Σ V)
       (pc2 : TT2 → V * iProp Σ * iProto Σ V) :
     ▷ (∀.. x1 : TT1, (pc1 x1).1.2 -∗ ∃.. x2 : TT2,
       ⌜(pc1 x1).1.1 = (pc2 x2).1.1⌝ ∗
@@ -693,37 +628,15 @@ Section proto.
       iProto_le (pc1 x1).2 (pc2 x2).2) -∗
     iProto_le (iProto_message Recv pc1) (iProto_message Recv pc2).
   Proof.
-    iIntros "H". iApply iProto_le_recv. iIntros (x2) "Hpc".
-    rewrite bi_tforall_forall. iDestruct ("H" with "Hpc") as "H".
-    rewrite bi_texist_exist bi.later_exist_except_0.
-    iMod "H" as (x1) "(>% & Hpc & Hle)". iExists x1. by iFrame.
+    iIntros "H". rewrite iProto_le_unfold iProto_message_eq.
+    iRight. iExists _, _, _, _; do 2 (iSplit; [done|]).
+    iIntros "!>" (v p1') "/=". iDestruct 1 as (x1 ->) "[Hpc #Heq]".
+    iDestruct ("H" with "Hpc") as (x2 ?) "[Hpc Hle]".
+    iExists (pc2 x2).2. iSplitL "Hle"; [by iRewrite "Heq"|].
+    iExists x2. iSplit; [done|]. iSplit; [by iApply "Hpc"|done].
   Qed.
 
   Lemma iProto_le_swap {TT1 TT2} (pc1 : TT1 → V * iProp Σ * iProto Σ V)
-      (pc2 : TT2 → V * iProp Σ * iProto Σ V) :
-    (∀.. (x1 : TT1) (x2 : TT2),
-      ▷ (pc1 x1).1.2 -∗ ▷ (pc2 x2).1.2 -∗
-      ◇ ∃ {TT3 TT4} (pc3 : TT3 → V * iProp Σ * iProto Σ V)
-          (pc4 : TT4 → V * iProp Σ * iProto Σ V), ∃.. (x3 : TT3) (x4 : TT4),
-        ⌜(pc1 x1).1.1 = (pc4 x4).1.1⌝ ∗
-        ⌜(pc2 x2).1.1 = (pc3 x3).1.1⌝ ∗
-        ▷ iProto_le (pc1 x1).2 (iProto_message Send pc3) ∗
-        ▷ iProto_le (iProto_message Recv pc4) (pc2 x2).2 ∗
-        ▷ (pc3 x3).1.2 ∗ ▷ (pc4 x4).1.2 ∗
-        ▷ ((pc3 x3).2 ≡ (pc4 x4).2)) -∗
-    iProto_le (iProto_message Recv pc1) (iProto_message Send pc2).
-  Proof.
-    iIntros "H". rewrite iProto_le_unfold iProto_message_eq.
-    iRight. iExists _, _, _, _; do 2 (iSplit; [done|]); simpl.
-    iIntros (v1 v2 p1 p2).
-    iDestruct 1 as (x1 ->) "[Hpc1 #Heq1]"; iDestruct 1 as (x2 ->) "[Hpc2 #Heq2]".
-    iMod ("H" with "Hpc1 Hpc2")
-      as (TT3 TT4 pc3 pc4 x3 x4 ??) "(H1 & H2 & Hpc1 & Hpc2 & #H)".
-    iModIntro. iExists _, _, (pc3 x3).2. iSplitL "H1"; [iNext; by iRewrite "Heq1"|].
-    iSplitL "H2"; [iNext; by iRewrite "Heq2"|]. simpl.
-    iSplitL "Hpc1"; [by auto|]. iExists x4. rewrite !bi.later_equivI. auto.
-  Qed.
-  Lemma iProto_le_swap' {TT1 TT2} (pc1 : TT1 → V * iProp Σ * iProto Σ V)
       (pc2 : TT2 → V * iProp Σ * iProto Σ V) :
     ▷ (∀.. (x1 : TT1) (x2 : TT2),
       (pc1 x1).1.2 -∗ (pc2 x2).1.2 -∗
@@ -737,16 +650,14 @@ Section proto.
         ((pc3 x3).2 ≡ (pc4 x4).2)) -∗
     iProto_le (iProto_message Recv pc1) (iProto_message Send pc2).
   Proof.
-    iIntros "H". iApply iProto_le_swap. iIntros (x1 x2) "Hpc1 Hpc2".
-    repeat setoid_rewrite bi_tforall_forall. iDestruct ("H" with "Hpc1 Hpc2") as "H".
-    iMod (bi.later_exist_except_0 with "H") as (TT3) "H".
-    iMod (bi.later_exist_except_0 with "H") as (TT4) "H".
-    iMod (bi.later_exist_except_0 with "H") as (pc3) "H".
-    iMod (bi.later_exist_except_0 with "H") as (pc4) "H".
-    rewrite bi_texist_exist bi.later_exist_except_0. iMod "H" as (x3) "H".
-    rewrite bi_texist_exist bi.later_exist_except_0. iMod "H" as (x4) "H".
-    iDestruct "H" as "(>% & >% & H1 & H2 & Hpc1 & Hpc2 & #H)".
-    iExists TT3, TT4, pc3, pc4, x3, x4. iFrame. auto.
+    iIntros "H". rewrite iProto_le_unfold iProto_message_eq.
+    iRight. iExists _, _, _, _; do 2 (iSplit; [done|]); simpl.
+    iIntros "!>" (v1 v2 p1 p2).
+    iDestruct 1 as (x1 ->) "[Hpc1 #Heq1]"; iDestruct 1 as (x2 ->) "[Hpc2 #Heq2]".
+    iDestruct ("H" with "Hpc1 Hpc2")
+      as (TT3 TT4 pc3 pc4 x3 x4 ??) "(H1 & H2 & Hpc1 & Hpc2 & #H)".
+    iExists _, _, (pc3 x3).2. iSplitL "H1"; [by iRewrite "Heq1"|].
+    iSplitL "H2"; [by iRewrite "Heq2"|]. simpl. iSplitL "Hpc1"; eauto.
   Qed.
 
   Lemma iProto_le_swap_simple {TT1 TT2} (v1 : TT1 → V) (v2 : TT2 → V)
@@ -757,7 +668,7 @@ Section proto.
         (iProto_message Send (λ x2,
           (v2 x2, P2 x2, iProto_message Recv (λ x1, (v1 x1, P1 x1, p x1 x2))))).
   Proof.
-    iApply iProto_le_swap. iIntros (x1 x2) "/= HP1 HP2".
+    iApply iProto_le_swap. iIntros "!>" (x1 x2) "/= HP1 HP2".
     iExists TT2, TT1, (λ x2, (v2 x2, P2 x2, p x1 x2)),
       (λ x1, (v1 x1, P1 x1, p x1 x2)), x2, x1; simpl.
     do 2 (iSplit; [done|]). do 2 (iSplitR; [iApply iProto_le_refl|]). by iFrame.
@@ -773,28 +684,25 @@ Section proto.
       iRewrite "Hp2"; clear p2. iEval (rewrite !iProto_dual_message').
       rewrite iProto_le_unfold; iRight.
       iExists _, _, _, _; do 2 (iSplit; [done|]); simpl. destruct a2; simpl.
-      + iIntros (v p1d). iDestruct 1 as (p1') "[Hpc #Hp1d]".
-        iMod ("H" with "Hpc") as (p2') "[H Hpc]".
+      + iIntros "!>" (v p1d). iDestruct 1 as (p1') "[Hpc #Hp1d]".
+        iDestruct ("H" with "Hpc") as (p2') "[H Hpc]".
         iDestruct ("IH" with "H") as "H".
-        iModIntro. iExists (iProto_dual p2'). iSplitR "Hpc"; [|by auto].
-        iNext. by iRewrite "Hp1d".
-      + iIntros (v1 v2 p1d p2d).
+        iExists (iProto_dual p2'). iSplitR "Hpc"; [|by auto]. by iRewrite "Hp1d".
+      + iIntros "!>" (v1 v2 p1d p2d).
         iDestruct 1 as (p1') "[Hpc1 #Hp1d]". iDestruct 1 as (p2') "[Hpc2 #Hp2d]".
-        iMod ("H" with "Hpc2 Hpc1") as (pc1' pc2' pt) "(H1 & H2 & Hpc1 & Hpc2)".
+        iDestruct ("H" with "Hpc2 Hpc1") as (pc1' pc2' pt) "(H1 & H2 & Hpc1 & Hpc2)".
         iDestruct ("IH" with "H1") as "H1". iDestruct ("IH" with "H2") as "H2 {IH}".
-        rewrite !iProto_dual_message' /=. iModIntro. iExists _, _, (iProto_dual pt).
-        iSplitL "H2"; [iNext; by iRewrite "Hp1d"|].
-        iSplitL "H1"; [iNext; by iRewrite "Hp2d"|].
+        rewrite !iProto_dual_message' /=. iExists _, _, (iProto_dual pt).
+        iSplitL "H2"; [by iRewrite "Hp1d"|]. iSplitL "H1"; [by iRewrite "Hp2d"|].
         iSplitL "Hpc2"; simpl; auto.
     - iDestruct (iProto_le_recv_inv with "H") as (pc2) "[Hp2 H]".
       iRewrite "Hp2"; clear p2. iEval (rewrite !iProto_dual_message' /=).
       rewrite iProto_le_unfold; iRight.
       iExists _, _, _, _; do 2 (iSplit; [done|]); simpl.
-      iIntros (v p2d). iDestruct 1 as (p2') "[Hpc #Hp2d]".
-      iMod ("H" with "Hpc") as (p1') "[H Hpc]".
+      iIntros "!>" (v p2d). iDestruct 1 as (p2') "[Hpc #Hp2d]".
+      iDestruct ("H" with "Hpc") as (p1') "[H Hpc]".
       iDestruct ("IH" with "H") as "H".
-      iModIntro. iExists (iProto_dual p1'). iSplitR "Hpc"; [|by auto].
-      iNext. by iRewrite "Hp2d".
+      iExists (iProto_dual p1'). iSplitR "Hpc"; [|by auto]. by iRewrite "Hp2d".
   Qed.
 
   Lemma iProto_le_dual_l p1 p2 :
@@ -803,7 +711,6 @@ Section proto.
     iIntros "H". iEval (rewrite -(involutive iProto_dual p2)).
     by iApply iProto_le_dual.
   Qed.
-
   Lemma iProto_le_dual_r p1 p2 :
     iProto_le p2 (iProto_dual p1) -∗ iProto_le p1 (iProto_dual p2).
   Proof.
@@ -821,30 +728,28 @@ Section proto.
       iRewrite "Hp1"; clear p1.
       rewrite !iProto_app_message'. iEval (rewrite iProto_le_unfold).
       iRight. iExists _, _, _, _; do 2 (iSplit; [done|]). destruct a1; simpl.
-      + iIntros (v p24). iDestruct 1 as (p2') "[Hpc #Hp24]".
-        iMod ("H1" with "Hpc") as (p1') "[H1 Hpc]". iIntros "!>".
+      + iIntros "!>" (v p24). iDestruct 1 as (p2') "[Hpc #Hp24]".
+        iDestruct ("H1" with "Hpc") as (p1') "[H1 Hpc]".
         iExists (p1' <++> p3)%proto. iSplitR "Hpc"; [|eauto].
-        iIntros "!>". iRewrite "Hp24". by iApply ("IH" with "H1").
-      + iIntros (v1 v2 p13 p24).
+        iRewrite "Hp24". by iApply ("IH" with "H1").
+      + iIntros "!>" (v1 v2 p13 p24).
         iDestruct 1 as (p1') "[Hpc1 #Hp13]"; iDestruct 1 as (p2') "[Hpc2 #Hp24]".
-        iMod ("H1" with "Hpc1 Hpc2") as (pc1' pc2' pt) "(H1 & H1' & Hpc1 & Hpc2)".
-        iIntros "!>".
-        iExists (iProto_map_cont (flip iProto_app p3) ∘ pc1'),
-          (iProto_map_cont (flip iProto_app p3) ∘ pc2'), (pt <++> p3)%proto.
+        iDestruct ("H1" with "Hpc1 Hpc2") as (pc1' pc2' pt) "(H1 & H1' & Hpc1 & Hpc2)".
+        iExists (iProto_map_app_cont (flip iProto_app p3) ∘ pc1'),
+          (iProto_map_app_cont (flip iProto_app p3) ∘ pc2'), (pt <++> p3)%proto.
         rewrite -!iProto_app_message' /=. iSplitL "H1".
-        { iIntros "!>". iRewrite "Hp13". iApply ("IH" with "H1").
-          iApply iProto_le_refl. }
+        { iRewrite "Hp13". iApply ("IH" with "H1"). iApply iProto_le_refl. }
         iSplitL "H2 H1'".
-        { iIntros "!>". iRewrite "Hp24". iApply ("IH" with "H1' H2"). }
+        { iRewrite "Hp24". iApply ("IH" with "H1' H2"). }
         iSplitL "Hpc1"; auto.
     - iDestruct (iProto_le_recv_inv with "H1") as (pc1) "[Hp1 H1]".
       iRewrite "Hp1"; clear p1.
       rewrite !iProto_app_message'. iEval (rewrite iProto_le_unfold).
       iRight. iExists _, _, _, _; do 2 (iSplit; [done|]); simpl.
-      iIntros (v p13). iDestruct 1 as (p1') "[Hpc #Hp13]".
-      iMod ("H1" with "Hpc") as (p2'') "[H1 Hpc]". iIntros "!>".
+      iIntros "!>" (v p13). iDestruct 1 as (p1') "[Hpc #Hp13]".
+      iDestruct ("H1" with "Hpc") as (p2'') "[H1 Hpc]".
       iExists (p2'' <++> p4)%proto. iSplitR "Hpc"; [|eauto].
-      iIntros "!>". iRewrite "Hp13". by iApply ("IH" with "H1").
+      iRewrite "Hp13". by iApply ("IH" with "H1").
   Qed.
 
   (** ** Lemmas about the auxiliary definitions and invariants *)
@@ -907,12 +812,12 @@ Section proto.
       (∃ vl vsl' pc pr',
         ⌜ vsl = vl :: vsl' ⌝ ∗
         iProto_le (proto_message Recv pc) pr ∗
-        pc vl (Next pr') ∗
+        pc vl pr' ∗
         iProto_interp vsl' vsr pl pr') ∨
       (∃ vr vsr' pc pl',
         ⌜ vsr = vr :: vsr' ⌝ ∗
         iProto_le (proto_message Recv pc) pl ∗
-        pc vr (Next pl') ∗
+        pc vr pl' ∗
         iProto_interp vsl vsr' pl' pr).
   Proof.
     rewrite {1}/iProto_interp. destruct vsl as [|vl vsl]; simpl.
@@ -979,7 +884,7 @@ Section proto.
   Lemma iProto_interp_send vl pcl vsl vsr pl pr pl' :
     iProto_interp vsl vsr pl pr -∗
     iProto_le pl (proto_message Send pcl) -∗
-    pcl vl (Next pl') -∗
+    pcl vl pl' -∗
     ▷^(length vsr) iProto_interp (vsl ++ [vl]) vsr pl' pr.
   Proof.
     iIntros "H Hle". iDestruct (iProto_interp_le_l with "H Hle") as "H".
@@ -1002,10 +907,10 @@ Section proto.
     - iDestruct "H" as (vr' vsr' pc' pl'' ->) "(Hle & Hpcl' & H) /=".
       iDestruct (iProto_le_send_inv with "Hle") as (a pcl') "[Hpc Hle]".
       iDestruct (proto_message_equivI with "Hpc") as (<-) "Hpc".
-      iRewrite ("Hpc" $! vr' (Next pl'')) in "Hpcl'"; clear pc'.
-      iMod ("Hle" with "Hpcl' Hpcl")
+      iIntros "!>". iRewrite ("Hpc" $! vr' pl'') in "Hpcl'"; clear pc'.
+      iDestruct ("Hle" with "Hpcl' Hpcl")
         as (pc1 pc2 pt) "(Hpl'' & Hpl' & Hpc1 & Hpc2)".
-      iNext. iDestruct (iProto_interp_le_l with "H Hpl''") as "H".
+      iDestruct (iProto_interp_le_l with "H Hpl''") as "H".
       iDestruct ("IH" with "[%] [//] H Hpc1") as "H"; [simpl; lia|..].
       iNext. iApply iProto_interp_unfold. iRight; iRight.
       iExists vr', vsr', _, pt. iSplit; [done|]. by iFrame.
@@ -1014,7 +919,7 @@ Section proto.
   Lemma iProto_interp_recv vl vsl vsr pl pr pcr :
     iProto_interp (vl :: vsl) vsr pl pr -∗
     iProto_le pr (proto_message Recv pcr) -∗
-    ◇ ∃ pr, pcr vl (Next pr) ∗ ▷ iProto_interp vsl vsr pl pr.
+    ▷ ∃ pr, pcr vl pr ∗ iProto_interp vsl vsr pl pr.
   Proof.
     iIntros "H Hle". iDestruct (iProto_interp_le_r with "H Hle") as "H".
     clear pr. remember (length vsr) as n eqn:Hn.
@@ -1024,13 +929,14 @@ Section proto.
     - iClear "IH". iDestruct "H" as (vl' vsl' pc' pr' [= -> ->]) "(Hpr & Hpc' & Hinterp)".
       iDestruct (iProto_le_recv_inv with "Hpr") as (pc'') "[Hpc Hpr]".
       iDestruct (proto_message_equivI with "Hpc") as (_) "{Hpc} #Hpc".
-      iMod ("Hpr" $! vl' pr' with "[Hpc']") as (pr'') "[Hler Hpr]".
-      { by iRewrite -("Hpc" $! vl' (Next pr')). }
-      iModIntro. iExists pr''. iFrame "Hpr".
+      iIntros "!>".
+      iDestruct ("Hpr" $! vl' pr' with "[Hpc']") as (pr'') "[Hler Hpr]".
+      { by iRewrite -("Hpc" $! vl' pr'). }
+      iExists pr''. iFrame "Hpr".
       by iApply (iProto_interp_le_r with "Hinterp").
     - iDestruct "H" as (vr vsr' pc' pl'' ->) "(Hpl & Hpc' & Hinterp)".
-      iMod ("IH" with "[%] [//] Hinterp") as (pr) "[Hpc Hinterp]"; [simpl; lia|].
-      iModIntro. iExists pr. iFrame "Hpc".
+      iDestruct ("IH" with "[%] [//] Hinterp") as (pr) "[Hpc Hinterp]"; [simpl; lia|].
+      iIntros "!>". iExists pr. iFrame "Hpc".
       iApply iProto_interp_unfold. iRight; iRight. eauto 20 with iFrame.
   Qed.
 
@@ -1119,7 +1025,8 @@ Section proto.
     iDestruct (iProto_interp_recv with "Hinterp [Hle]") as (q) "[Hpc Hinterp]".
     { iNext. by iRewrite "Hp". }
     iMod (iProto_own_auth_update _ _ _ _ q with "H●l H◯") as "[H●l H◯]".
-    iIntros "!> !>". iMod "Hinterp". iMod "Hpc" as (x ->) "[Hpc #Hq] /=".
+    iIntros "!> !> /=".
+    iMod (bi.later_exist_except_0 with "Hpc") as (x) "(>-> & Hpc & #Hq)".
     iIntros "!>". iExists x. iSplit; [done|]. iFrame "Hpc". iSplitR "H◯".
     - iExists q, pr. iFrame. by iApply iProto_interp_flip.
     - iExists q. iIntros "{$H◯} !>". iRewrite "Hq". iApply iProto_le_refl.
@@ -1140,7 +1047,8 @@ Section proto.
     iDestruct (iProto_interp_recv with "Hinterp [Hle]") as (q) "[Hpc Hinterp]".
     { iNext. by iRewrite "Hp". }
     iMod (iProto_own_auth_update _ _ _ _ q with "H●r H◯") as "[H●r H◯]".
-    iIntros "!> !>". iMod "Hinterp". iMod "Hpc" as (x ->) "[Hpc #Hq] /=".
+    iIntros "!> !> /=".
+    iMod (bi.later_exist_except_0 with "Hpc") as (x) "(>-> & Hpc & #Hq)".
     iIntros "!>". iExists x. iSplit; [done|]. iFrame "Hpc". iSplitR "H◯".
     - iExists pl, q. iFrame.
     - iExists q. iIntros "{$H◯} !>". iRewrite "Hq". iApply iProto_le_refl.
